src/Lean/Meta/Tactic/Simp/SimpLemmas.lean
@@ -14,6 +14,7 @@ structure SimpLemma where
   keys     : Array DiscrTree.Key
   val      : Expr
   priority : Nat
+  post     : Bool
   perm     : Bool -- true is lhs and rhs are identical modulo permutation of variables
   name?    : Option Name := none -- for debugging and tracing purposes
   deriving Inhabited
@@ -32,11 +33,15 @@ instance : BEq SimpLemma where
   beq e₁ e₂ := e₁.val == e₂.val
 
 structure SimpLemmas where
-  discrTree       : DiscrTree SimpLemma := DiscrTree.empty
+  pre  : DiscrTree SimpLemma := DiscrTree.empty
+  post : DiscrTree SimpLemma := DiscrTree.empty
   deriving Inhabited
 
 def addSimpLemmaEntry (d : SimpLemmas) (e : SimpLemma) : SimpLemmas :=
-  { d with discrTree := d.discrTree.insertCore e.keys e }
+  if e.post then
+    { d with post := d.post.insertCore e.keys e }
+  else
+    { d with pre := d.pre.insertCore e.keys e }
 
 builtin_initialize simpExtension : SimpleScopedEnvExtension SimpLemma SimpLemmas ←
   registerSimpleScopedEnvExtension {
@@ -57,7 +62,7 @@ private partial def isPerm : Expr → Expr → MetaM Bool
   | Expr.proj _ i₁ b₁ _, Expr.proj _ i₂ b₂ _ => i₁ == i₂ <&&> isPerm b₁ b₂
   | s, t => s == t
 
-def mkSimpLemmaCore (e : Expr) (val : Expr) (prio : Nat) (name? : Option Name) : MetaM SimpLemma := do
+def mkSimpLemmaCore (e : Expr) (val : Expr) (post : Bool) (prio : Nat) (name? : Option Name) : MetaM SimpLemma := do
   let type ← inferType e
   unless (← isProp type) do
     throwError! "invalid 'simp', proposition expected{indentExpr type}"
@@ -77,12 +82,12 @@ def mkSimpLemmaCore (e : Expr) (val : Expr) (prio : Nat) (name? : Option Name) :
             pure (← DiscrTree.mkPath (← inferType xs.back), false)
         else
           pure (← DiscrTree.mkPath type, false)
-    return { keys := keys, perm := perm, val := val, name? := name?, priority := prio }
+    return { keys := keys, perm := perm, post := post, val := val, name? := name?, priority := prio }
 
-def addSimpLemma (declName : Name) (attrKind : AttributeKind) (prio : Nat) : MetaM Unit := do
+def addSimpLemma (declName : Name) (post : Bool) (attrKind : AttributeKind) (prio : Nat) : MetaM Unit := do
   let cinfo ← getConstInfo declName
   /- The `simp` tactic uses fresh universe metavariables when using a global simp lemma. -/
-  let lemma ← mkSimpLemmaCore (mkConst declName (cinfo.lparams.map mkLevelParam)) (mkConst declName) prio declName
+  let lemma ← mkSimpLemmaCore (mkConst declName (cinfo.lparams.map mkLevelParam)) (mkConst declName) post prio declName
   simpExtension.add lemma attrKind
   pure ()
 
@@ -91,20 +96,25 @@ builtin_initialize
     name  := `simp
     descr := "simplification lemma"
     add   := fun declName stx attrKind => do
-      let prio ← getAttrParamOptPrio stx[1]
-      discard <| addSimpLemma declName attrKind prio |>.run {} {}
+      let post :=
+        if stx[1].isNone then true else stx[1][0].getKind == ``Lean.Parser.Tactic.simpPost
+      let prio ← getAttrParamOptPrio stx[2]
+      discard <| addSimpLemma declName post attrKind prio |>.run {} {}
   }
 
-def getSimpLemmas : MetaM (DiscrTree SimpLemma) :=
-  return simpExtension.getState (← getEnv) |>.discrTree
+def getPreSimpLemmas : MetaM (DiscrTree SimpLemma) :=
+  return simpExtension.getState (← getEnv) |>.pre
+
+def getPostSimpLemmas : MetaM (DiscrTree SimpLemma) :=
+  return simpExtension.getState (← getEnv) |>.post
 
 /- Auxiliary method for creating a local simp lemma. -/
-def mkSimpLemma (e : Expr) (prio : Nat := evalPrio! default) (name? : Option Name := none) : MetaM SimpLemma := do
-  mkSimpLemmaCore e e prio name?
+def mkSimpLemma (e : Expr) (post : Bool := true) (prio : Nat := evalPrio! default) (name? : Option Name := none) : MetaM SimpLemma := do
+  mkSimpLemmaCore e e post prio name?
 
 /- Auxiliary method for adding a local simp lemma to a `SimpLemmas` datastructure. -/
-def SimpLemmas.add (s : SimpLemmas) (e : Expr) (prio : Nat := evalPrio! default) (name? : Option Name := none) : MetaM SimpLemmas := do
-  let lemma ← mkSimpLemma e prio name?
+def SimpLemmas.add (s : SimpLemmas) (e : Expr) (post : Bool := true) (prio : Nat := evalPrio! default) (name? : Option Name := none) : MetaM SimpLemmas := do
+  let lemma ← mkSimpLemma e post prio name?
   return addSimpLemmaEntry s lemma
 
 end Lean.Meta
